spec/Rchain.lean
@@ -27,6 +27,7 @@ import Rchain.RSpace.Comm
 import Rchain.RSpace.Merge
 import Rchain.RSpace.Merkle
 import Rchain.Casper.Stake
+import Rchain.Proto
 import Rchain.Casper.Fringe
 import Rchain.Casper.Validate
 import Rchain.Pos
